thys/Resolution_FOL/TermsAndLiterals.thy
@@ -1,4 +1,4 @@
-section{* Terms and Literals *}
+section \<open>Terms and Literals\<close>
 
 theory TermsAndLiterals imports Main "HOL-Library.Countable_Set" begin
 
@@ -23,7 +23,8 @@ fun get_atom :: "'t literal \<Rightarrow> 't atom" where
   "get_atom (Pos p ts) = (p, ts)"
 | "get_atom (Neg p ts) = (p, ts)"
 
-subsection {* Ground *}
+
+subsection \<open>Ground\<close>
 
 fun ground\<^sub>t :: "fterm \<Rightarrow> bool" where
   "ground\<^sub>t (Var x) \<longleftrightarrow> False"
@@ -37,15 +38,17 @@ abbreviation ground\<^sub>l :: "fterm literal \<Rightarrow> bool" where
 
 abbreviation ground\<^sub>l\<^sub>s :: "fterm literal set \<Rightarrow> bool" where
   "ground\<^sub>l\<^sub>s C \<equiv> (\<forall>l \<in> C. ground\<^sub>l l)"
-
-
+  
 definition ground_fatoms :: "fterm atom set" where
   "ground_fatoms \<equiv> {a. ground\<^sub>t\<^sub>s (snd a)}"
 
-lemma ground\<^sub>l_ground_fatom: "ground\<^sub>l l \<Longrightarrow> get_atom l \<in> ground_fatoms"
-  unfolding ground_fatoms_def by (induction l) auto
+lemma ground\<^sub>l_ground_fatom: 
+  assumes "ground\<^sub>l l"
+  shows "get_atom l \<in> ground_fatoms"
+  using assms unfolding ground_fatoms_def by (induction l) auto
 
-subsection {* Auxiliary *}
+
+subsection \<open>Auxiliary\<close>
 
 lemma infinity:
   assumes inj: "\<forall>n :: nat. undiago (diago n) = n" 
@@ -70,8 +73,11 @@ lemma f_inv_into_f:
   shows "f ((inv_into A f) b) = b"
 using assms bij_betw_inv_into_right by metis
 
-subsection {* Conversions *}
-subsubsection {* Convertions - Terms and Herbrand Terms *}
+
+subsection \<open>Conversions\<close>
+
+
+subsubsection \<open>Conversions - Terms and Herbrand Terms\<close>
 
 fun fterm_of_hterm :: "hterm \<Rightarrow> fterm" where
   "fterm_of_hterm (HFun p ts) = Fun p (map fterm_of_hterm ts)"
@@ -85,17 +91,21 @@ fun hterm_of_fterm :: "fterm \<Rightarrow> hterm" where
 definition hterms_of_fterms :: "fterm list \<Rightarrow> hterm list" where
 "hterms_of_fterms ts \<equiv> map hterm_of_fterm ts"
 
-lemma [simp]: "hterm_of_fterm (fterm_of_hterm t) = t" 
+lemma hterm_of_fterm_fterm_of_hterm[simp]: "hterm_of_fterm (fterm_of_hterm t) = t" 
   by (induction t) (simp add: map_idI)
 
-lemma [simp]: "hterms_of_fterms (fterms_of_hterms ts) = ts" 
+lemma hterms_of_fterms_fterms_of_hterms[simp]: "hterms_of_fterms (fterms_of_hterms ts) = ts" 
   unfolding hterms_of_fterms_def fterms_of_hterms_def by (simp add: map_idI)
 
-lemma [simp]: "ground\<^sub>t t \<Longrightarrow> fterm_of_hterm (hterm_of_fterm t) = t" 
-  by (induction t) (auto simp add: map_idI)
+lemma fterm_of_hterm_hterm_of_fterm[simp]:
+  assumes "ground\<^sub>t t"
+  shows "fterm_of_hterm (hterm_of_fterm t) = t" 
+  using assms by (induction t) (auto simp add: map_idI)
 
-lemma [simp]: "ground\<^sub>t\<^sub>s ts \<Longrightarrow> fterms_of_hterms (hterms_of_fterms ts) = ts" 
-  unfolding fterms_of_hterms_def hterms_of_fterms_def by (simp add: map_idI)
+lemma fterms_of_hterms_hterms_of_fterms[simp]: 
+  assumes "ground\<^sub>t\<^sub>s ts"
+  shows "fterms_of_hterms (hterms_of_fterms ts) = ts" 
+  using assms unfolding fterms_of_hterms_def hterms_of_fterms_def by (simp add: map_idI)
 
 lemma ground_fterm_of_hterm:  "ground\<^sub>t (fterm_of_hterm t)"
   by (induction t) (auto simp add: map_idI)
@@ -103,7 +113,8 @@ lemma ground_fterm_of_hterm:  "ground\<^sub>t (fterm_of_hterm t)"
 lemma ground_fterms_of_hterms: "ground\<^sub>t\<^sub>s (fterms_of_hterms ts)"
   unfolding fterms_of_hterms_def using ground_fterm_of_hterm by auto
 
-subsubsection {* Conversions -  Literals and Herbrand Literals *}
+
+subsubsection \<open>Conversions -  Literals and Herbrand Literals\<close>
 
 fun flit_of_hlit :: "hterm literal \<Rightarrow> fterm literal" where
   "flit_of_hlit (Pos p ts) = Pos p (fterms_of_hterms ts)"
@@ -118,7 +129,10 @@ lemma ground_flit_of_hlit: "ground\<^sub>l (flit_of_hlit l)"
 
 theorem hlit_of_flit_flit_of_hlit [simp]: "hlit_of_flit (flit_of_hlit l) =  l" by (cases l) auto
 
-theorem flit_of_hlit_hlit_of_flit [simp]: "ground\<^sub>l l \<Longrightarrow> flit_of_hlit (hlit_of_flit l) = l" by (cases l) auto
+theorem flit_of_hlit_hlit_of_flit [simp]:
+  assumes "ground\<^sub>l l"
+  shows "flit_of_hlit (hlit_of_flit l) = l"
+  using assms by (cases l) auto
 
 lemma sign_flit_of_hlit: "sign (flit_of_hlit l) = sign l" by (cases l) auto
 
@@ -146,7 +160,8 @@ next
   ultimately show "flit_of_hlit ` UNIV = {l. ground\<^sub>l l}" using hlit_of_flit_flit_of_hlit ground_flit_of_hlit by auto
 qed
 
-subsubsection {* Convertions - Atoms and Herbrand Atoms *}
+
+subsubsection \<open>Conversions - Atoms and Herbrand Atoms\<close>
 
 fun fatom_of_hatom :: "hterm atom \<Rightarrow> fterm atom" where
   "fatom_of_hatom (p, ts) = (p, fterms_of_hterms ts)"
@@ -157,9 +172,13 @@ fun hatom_of_fatom :: "fterm atom \<Rightarrow> hterm atom" where
 lemma ground_fatom_of_hatom: "ground\<^sub>t\<^sub>s (snd (fatom_of_hatom a))" 
   by  (induction a) (simp add: ground_fterms_of_hterms)+
 
-theorem hatom_of_fatom_fatom_of_hatom [simp]: "hatom_of_fatom (fatom_of_hatom l) = l" by (cases l) auto
+theorem hatom_of_fatom_fatom_of_hatom [simp]: "hatom_of_fatom (fatom_of_hatom l) = l" 
+  by (cases l) auto
 
-theorem fatom_of_hatom_hatom_of_fatom [simp]: "ground\<^sub>t\<^sub>s (snd l) \<Longrightarrow> fatom_of_hatom (hatom_of_fatom l) = l" by (cases l) auto
+theorem fatom_of_hatom_hatom_of_fatom [simp]: 
+  assumes "ground\<^sub>t\<^sub>s (snd l)"
+  shows "fatom_of_hatom (hatom_of_fatom l) = l"
+  using assms by (cases l) auto
 
 lemma hatom_of_fatom_bij: "bij_betw hatom_of_fatom ground_fatoms UNIV" 
  unfolding bij_betw_def
@@ -187,101 +206,104 @@ next
 qed
 
 
-subsection {* Enumerations *}
+subsection \<open>Enumerations\<close>
 
-subsubsection {* Enumerating Strings *}
 
-definition nat_from_string:: "string \<Rightarrow> nat" where
-  "nat_from_string \<equiv> (SOME f. bij f)"
+subsubsection \<open>Enumerating Strings\<close>
 
-definition string_from_nat:: "nat \<Rightarrow> string" where
-  "string_from_nat \<equiv> inv nat_from_string"
+definition nat_of_string:: "string \<Rightarrow> nat" where
+  "nat_of_string \<equiv> (SOME f. bij f)"
 
-lemma nat_from_string_bij: "bij nat_from_string"
+definition string_of_nat:: "nat \<Rightarrow> string" where
+  "string_of_nat \<equiv> inv nat_of_string"
+
+lemma nat_of_string_bij: "bij nat_of_string"
   proof -
   have "countable (UNIV::string set)" by auto
   moreover
   have "infinite (UNIV::string set)" using infinite_UNIV_listI by auto
   ultimately
   obtain x where "bij (x:: string \<Rightarrow> nat)" using countableE_infinite[of UNIV] by blast
-  then show "?thesis" unfolding nat_from_string_def using someI by metis
+  then show "?thesis" unfolding nat_of_string_def using someI by metis
 qed
 
-lemma string_from_nat_bij: "bij string_from_nat" unfolding string_from_nat_def using nat_from_string_bij bij_betw_inv_into by auto
+lemma string_of_nat_bij: "bij string_of_nat" unfolding string_of_nat_def using nat_of_string_bij bij_betw_inv_into by auto
 
-lemma nat_from_string_string_from_nat[simp]: "nat_from_string (string_from_nat n) = n" 
-  unfolding string_from_nat_def 
-  using nat_from_string_bij f_inv_into_f[of nat_from_string] by simp
+lemma nat_of_string_string_of_nat[simp]: "nat_of_string (string_of_nat n) = n" 
+  unfolding string_of_nat_def 
+  using nat_of_string_bij f_inv_into_f[of nat_of_string] by simp
 
-lemma string_from_nat_nat_from_string[simp]: "string_from_nat (nat_from_string n) = n" 
-  unfolding string_from_nat_def 
-  using nat_from_string_bij inv_into_f_f[of nat_from_string] by simp
+lemma string_of_nat_nat_of_string[simp]: "string_of_nat (nat_of_string n) = n" 
+  unfolding string_of_nat_def 
+  using nat_of_string_bij inv_into_f_f[of nat_of_string] by simp
 
-subsubsection {* Enumerating Herbrand Atoms *}
 
-definition nat_from_hatom:: "hterm atom \<Rightarrow> nat" where
-  "nat_from_hatom \<equiv> (SOME f. bij f)"
+subsubsection \<open>Enumerating Herbrand Atoms\<close>
 
-definition hatom_from_nat:: "nat \<Rightarrow> hterm atom" where
-  "hatom_from_nat \<equiv> inv nat_from_hatom"
+definition nat_of_hatom:: "hterm atom \<Rightarrow> nat" where
+  "nat_of_hatom \<equiv> (SOME f. bij f)"
+
+definition hatom_of_nat:: "nat \<Rightarrow> hterm atom" where
+  "hatom_of_nat \<equiv> inv nat_of_hatom"
 
 instantiation hterm :: countable begin
 instance by countable_datatype
 end
 
-lemma infinite_hatoms: "infinite (UNIV :: (pred_sym * 't list) set)"
+lemma infinite_hatoms: "infinite (UNIV :: ('t atom) set)"
 proof -
-  let ?diago = "\<lambda>n. (string_from_nat n,[])"
-  let ?undiago = "\<lambda>a. nat_from_string (fst a)"
-  have "\<forall>n. ?undiago (?diago n) = n" using nat_from_string_string_from_nat by auto
+  let ?diago = "\<lambda>n. (string_of_nat n,[])"
+  let ?undiago = "\<lambda>a. nat_of_string (fst a)"
+  have "\<forall>n. ?undiago (?diago n) = n" using nat_of_string_string_of_nat by auto
   moreover
   have "\<forall>n. ?diago n \<in> UNIV" by auto
-  ultimately show "infinite (UNIV :: (pred_sym * 't list) set)" using infinity[of ?undiago ?diago UNIV] by simp
+  ultimately show "infinite (UNIV :: ('t atom) set)" using infinity[of ?undiago ?diago UNIV] by simp
 qed
 
-lemma nat_from_hatom_bij: "bij nat_from_hatom"
+lemma nat_of_hatom_bij: "bij nat_of_hatom"
 proof -
-  let ?S = "UNIV :: (pred_sym * ('t::countable) list) set"
+  let ?S = "UNIV :: (('t::countable) atom) set"
   have "countable ?S" by auto
   moreover
   have "infinite ?S" using infinite_hatoms by auto
   ultimately
   obtain x where "bij (x :: hterm atom \<Rightarrow> nat)" using countableE_infinite[of ?S] by blast
-  then have "bij nat_from_hatom" unfolding nat_from_hatom_def using someI by metis
-  then show "?thesis" unfolding bij_betw_def inj_on_def unfolding nat_from_hatom_def by simp
+  then have "bij nat_of_hatom" unfolding nat_of_hatom_def using someI by metis
+  then show "?thesis" unfolding bij_betw_def inj_on_def unfolding nat_of_hatom_def by simp
 qed
 
-lemma hatom_from_nat_bij: "bij hatom_from_nat " unfolding hatom_from_nat_def using nat_from_hatom_bij bij_betw_inv_into by auto
+lemma hatom_of_nat_bij: "bij hatom_of_nat" unfolding hatom_of_nat_def using nat_of_hatom_bij bij_betw_inv_into by auto
 
-lemma nat_from_hatom_hatom_from_nat[simp]: "nat_from_hatom (hatom_from_nat n) = n" 
-  unfolding hatom_from_nat_def 
-  using nat_from_hatom_bij f_inv_into_f[of nat_from_hatom] by simp
+lemma nat_of_hatom_hatom_of_nat[simp]: "nat_of_hatom (hatom_of_nat n) = n" 
+  unfolding hatom_of_nat_def 
+  using nat_of_hatom_bij f_inv_into_f[of nat_of_hatom] by simp
 
-lemma hatom_from_nat_nat_from_hatom[simp]: "hatom_from_nat (nat_from_hatom l) = l" 
-  unfolding hatom_from_nat_def 
-  using nat_from_hatom_bij inv_into_f_f[of nat_from_hatom _ UNIV] by simp
-
-
-subsubsection {* Enumerating Ground Atoms *}
-
-definition fatom_from_nat :: "nat \<Rightarrow> fterm atom" where
-  "fatom_from_nat = (\<lambda>n. fatom_of_hatom (hatom_from_nat n))"
-
-definition nat_from_fatom :: "fterm atom \<Rightarrow> nat" where
-  "nat_from_fatom = (\<lambda>t. nat_from_hatom (hatom_of_fatom t))"
-
-theorem diag_undiag_fatom[simp]: "ground\<^sub>t\<^sub>s ts \<Longrightarrow> fatom_from_nat (nat_from_fatom (p,ts)) = (p,ts)"
-unfolding fatom_from_nat_def nat_from_fatom_def by auto
-
-theorem undiag_diag_fatom[simp]: "nat_from_fatom (fatom_from_nat n) = n" unfolding fatom_from_nat_def nat_from_fatom_def by auto
-
-lemma fatom_from_nat_bij: "bij_betw fatom_from_nat UNIV ground_fatoms" 
-  using hatom_from_nat_bij bij_betw_trans fatom_of_hatom_bij hatom_from_nat_bij unfolding fatom_from_nat_def comp_def by blast
+lemma hatom_of_nat_nat_of_hatom[simp]: "hatom_of_nat (nat_of_hatom l) = l" 
+  unfolding hatom_of_nat_def 
+  using nat_of_hatom_bij inv_into_f_f[of nat_of_hatom _ UNIV] by simp
 
 
-lemma ground_fatom_from_nat: "ground\<^sub>t\<^sub>s (snd (fatom_from_nat x))" unfolding fatom_from_nat_def using ground_fatom_of_hatom by auto
+subsubsection \<open>Enumerating Ground Atoms\<close>
 
-lemma nat_from_fatom_bij: "bij_betw nat_from_fatom ground_fatoms UNIV"
-   using nat_from_hatom_bij bij_betw_trans hatom_of_fatom_bij hatom_from_nat_bij unfolding nat_from_fatom_def comp_def by blast
+definition fatom_of_nat :: "nat \<Rightarrow> fterm atom" where
+  "fatom_of_nat = (\<lambda>n. fatom_of_hatom (hatom_of_nat n))"
+
+definition nat_of_fatom :: "fterm atom \<Rightarrow> nat" where
+  "nat_of_fatom = (\<lambda>t. nat_of_hatom (hatom_of_fatom t))"
+
+theorem diag_undiag_fatom[simp]: 
+  assumes "ground\<^sub>t\<^sub>s ts"
+  shows "fatom_of_nat (nat_of_fatom (p,ts)) = (p,ts)"
+using assms unfolding fatom_of_nat_def nat_of_fatom_def by auto
+
+theorem undiag_diag_fatom[simp]: "nat_of_fatom (fatom_of_nat n) = n" unfolding fatom_of_nat_def nat_of_fatom_def by auto
+
+lemma fatom_of_nat_bij: "bij_betw fatom_of_nat UNIV ground_fatoms" 
+  using hatom_of_nat_bij bij_betw_trans fatom_of_hatom_bij hatom_of_nat_bij unfolding fatom_of_nat_def comp_def by blast
+
+lemma ground_fatom_of_nat: "ground\<^sub>t\<^sub>s (snd (fatom_of_nat x))" unfolding fatom_of_nat_def using ground_fatom_of_hatom by auto
+
+lemma nat_of_fatom_bij: "bij_betw nat_of_fatom ground_fatoms UNIV"
+   using nat_of_hatom_bij bij_betw_trans hatom_of_fatom_bij hatom_of_nat_bij unfolding nat_of_fatom_def comp_def by blast
 
 end
